# 7.3 Inverse Trig Substitution
$$\int \sqrt{1-x^2}dx=I$$
$$\theta=\sin^{-1}x$$
$$x=\sin\theta$$
$$dx=\cos\theta d\theta$$
$$I=\int\sqrt{1-\sin^2\theta}\cos\theta d\theta$$
$$=\int\sqrt{\cos\theta}\cos\theta d\theta$$
$$=\int\cos^2\theta d\theta$$
$$\int\frac{1+\cos2\theta}{2}d\theta$$
$$\frac{\theta}{2}+\frac{\sin2\theta}{4}+C$$
$$\frac{\sin^{-1}x}{2}+\frac{2\sin\theta\cos\theta}{4}+C$$
$$\frac{\sin^{-1}x}{2}\frac{2x*x}{4\sqrt{1-x^2}}+C$$
$$\frac{1}{2}[\sin^{-1}x+\frac{x^2}{\sqrt{1-x^2}}]+C$$
---
a|a
-|-
$\sqrt{a^2-x^2}$|$x=a\sin\theta$
$\sqrt{a^2+x^2}$|$x=a\tan\theta$
$\sqrt{x^2-a^2}$|$x=a\sec\theta$
